proofs/compiler/end_to_end.v
@@ -33,6 +33,7 @@ From ITree Require Import
 Import ITree.
 
 Require Import
+  equiv_extras
   rutt_extras
   xrutt
   xrutt_facts
@@ -69,6 +70,7 @@ Require Import
   compiler_proof
   it_compiler_proof
   it_compiler_proof_2
+  asm_gen_proof
 .
 Require allocation.
 
@@ -226,12 +228,8 @@ Definition handleE : Handler (RndEvent unit) Rnd :=
     let* bs := unif_rV (Z.to_nat len) in
     Ret (tt, wseq_of_wvec bs).
 
-Definition translateE : itree (RndEvent unit) ~> itree Rnd :=
+Definition to_Rnd : itree (RndEvent unit) ~> itree Rnd :=
   fun _ t => interp handleE t.
-
-Lemma eutt_translateE T (RR : T -> T -> Prop) :
-  Proper (eutt RR ==> eutt RR) (translateE (T := T)).
-Proof. exact: eutt_interp'. Qed.
 
 Context
   {reg regx xreg rflag cond asm_op extra_op : Type}
@@ -278,12 +276,13 @@ Section DEFS.
 Class JazzIParams :=
   {
     entries : seq funname;
-    mI : mem;
-    ripI : pointer;
-    rmI : regmap;
-    rxmI : regxmap;
-    xrmI : xregmap;
-    rfmI : rflagmap;
+    mS : mem;
+    mT : mem;
+    ripT : pointer;
+    rmT : regmap;
+    rxmT : regxmap;
+    xrmT : xregmap;
+    rfmT : rflagmap;
   }.
 
 Context
@@ -291,20 +290,6 @@ Context
   (q : asm_prog)
   {JP : JazzIParams}
 .
-
-(* Source needs a memory, target needs all the rest except syscall_state. *)
-Definition _Mo : choiceType := {choice asmmem}.
-
-Definition _mi : _Mo :=
-  {|
-    asm_rip := ripI;
-    asm_scs := tt;
-    asm_mem := mI;
-    asm_reg := rmI;
-    asm_regx := rxmI;
-    asm_xreg := xrmI;
-    asm_flag := rfmI;
-  |}.
 
 Record export_fn :=
   {
@@ -314,31 +299,39 @@ Record export_fn :=
     efn_fd_ok : get_fundef (p_funcs p) _fn = Some efn_fd;
   }.
 
-Definition _No : choiceType := {choice export_fn}.
+Definition JNo : choiceType := {choice export_fn}.
 
 (* Safety should be proven assuming only that the shape coincides with initial
    memory. *)
 Record valid_input o :=
   {
     _args :> values;
-    vi_safe : safe_on p o mI _args;
-    vi_def : res_defined_on p o mI _args;
-    (* for each array, give me an address with enough space *)
+    vi_safe : safe_on p o mS _args;
+    vi_def : res_defined_on p o mS _args;
+    vi_ptrs : seq pointer;
+    (*vi_ptrs_ok :
+       forall i,
+         oseq.onth _args i = Some (Varr _ _) ->
+         exists2 p,
+           seq.onth vi_ptrs i = Some p
+           & ;*)
   }.
 
-Definition _In (o : _No) : choiceType := {choice valid_input o}.
+Definition JIn (o : JNo) : choiceType := {choice valid_input o}.
 
-Definition _Out (o : _No) : choiceType := seq wseq.
+Definition JOut (o : JNo) : choiceType := seq wseq.
 
 Instance JazzI : OracleSystemInterface :=
   {|
-    No := _No;
-    In := _In;
-    Out := _Out;
+    No := JNo;
+    In := JIn;
+    Out := JOut;
   |}.
 
 (* -------------------------------------------------------------------------- *)
 (* Source oracle system *)
+
+Definition MoS : choiceType := {choice mem}.
 
 Definition wseq_of_val (v : value) : wseq :=
   match v with
@@ -351,64 +344,111 @@ Definition unmkfs (fs : fstate) : seq wseq * mem :=
   ([seq wseq_of_val v | v <- fs.(fvals) ], fs.(fmem)).
 
 Definition isem_unit_res
-  (o : _No) (i : _In o) (m : _Mo) : itree E (_Out o * _Mo) :=
-  let fs := mkfs m.(asm_mem) i in
+  (o : JNo) (i : JIn o) (m : MoS) : itree E (JOut o * MoS) :=
+  let fs := mkfs m i in
   let* fs' := isem_unit p o fs in
   let (r, m') := unmkfs fs' in
-  Ret (r, xm_with_mem m' m).
+  Ret (r, m').
 
 #[global] Arguments isem_unit_res : clear implicits.
 
-(* TODO Why doesn't [|>] work for [translateE]? *)
-Definition _OoS (o : _No) (i : _In o) (m : _Mo) : itree Rnd (_Out o * _Mo) :=
-  let* ores := translateE (isem_unit_res o i m |> interp_Err) in
+(* TODO Why doesn't [|>] work for [to_Rnd]? *)
+Definition OoS (o : JNo) (i : JIn o) (m : MoS) : itree Rnd (JOut o * MoS) :=
+  let* ores := to_Rnd (isem_unit_res o i m |> interp_Err) in
   if ores is ESok res then Ret res
-  else Ret ([::], _mi). (* absurd *)
+  else Ret ([::], mS). (* absurd *)
 
 Instance Source : OracleSystem JazzI :=
   {|
-    Mo := _Mo;
-    Oo := _OoS;
-    mi := _mi;
+    Mo := MoS;
+    Oo := OoS;
+    mi := mS;
   |}.
 
 (* -------------------------------------------------------------------------- *)
 (* Target oracle system *)
 
+Definition MoT : choiceType := {choice asmmem}.
+
+Definition xmT : asmmem :=
+  {|
+    asm_rip := ripT;
+    asm_scs := tt;
+    asm_mem := mT;
+    asm_reg := rmT;
+    asm_regx := rxmT;
+    asm_xreg := xrmT;
+    asm_flag := rfmT;
+  |}.
+
+Definition xm_write
+  (x : asm_typed_reg) (v : value) (ptr : pointer) (xm : asmmem) : exec asmmem :=
+  match x with
+  | ARReg r =>
+      if v is Varr _ a then
+        let m' := write_wseq xm.(asm_mem) ptr (wseq_of_arr a) in
+        ok (xm_with_mem m' xm)
+      else
+        Let w := to_word reg_size v in
+        ok (mem_write_reg MSB_CLEAR r w xm)
+  | ARegX rx =>
+      Let w := to_word reg_size v in
+      ok (mem_write_regx MSB_CLEAR rx w xm)
+  | AXReg xr =>
+      Let w := to_word xreg_size v in
+      ok (mem_write_xreg MSB_CLEAR xr w xm)
+  | ABReg f =>
+      Let b := to_bool v in
+      ok (mem_write_rflag xm f (Some b))
+  end.
+
 Definition xm_writes
-  (m : asmmem) (xs : seq asm_typed_reg) (args : values) : exec asmmem.
-Proof using. Admitted.
+  (m : asmmem)
+  (xs : seq asm_typed_reg)
+  (args : values)
+  (ptrs : seq pointer) :
+  exec asmmem :=
+  foldM (fun x => xm_write x.1.1 x.1.2 x.2) m (zip (zip xs args) ptrs).
 
-Definition mkxm (fn : funname) (m : asmmem) (args : values) : asmmem :=
+Definition mkxm
+  (fn : funname) (m : asmmem) (args : values) (ptrs : seq pointer) : asmmem :=
   if get_fundef (asm_funcs q) fn is Some xfd then
-    rdflt _mi (xm_writes m xfd.(asm_fd_arg) args)
-  else _mi. (* absurd *)
+    rdflt xmT (xm_writes m xfd.(asm_fd_arg) args ptrs)
+  else xmT. (* absurd *)
 
-Definition xm_read (m : asmmem) (x : asm_typed_reg) : value.
-Proof using. Admitted.
+Definition xm_read
+  (xm : asmmem) (x : asm_typed_reg) (ty : atype) (ptr : pointer) : wseq :=
+  if ty is aarr ws len then
+    let len' := Z.to_pos (arr_size ws len) in
+    read_wseq xm.(asm_mem) ptr len'
+  else wseq_of_val (get_typed_reg_value xm x).
 
-Definition xget_res (fn : funname) (m : asmmem) : seq wseq :=
-  if get_fundef (asm_funcs q) fn is Some xfd then
-    [seq wseq_of_val (xm_read m x) | x <- xfd.(asm_fd_res) ]
+Definition xget_res
+  (fn : funname) (m : asmmem) (ptrs : seq pointer) : seq wseq :=
+  if get_fundef p.(p_funcs) fn is Some fd then
+    if get_fundef q.(asm_funcs) fn is Some xfd then
+      [seq xm_read m x.1.1 x.1.2 x.2
+      | x <- zip (zip xfd.(asm_fd_res) fd.(f_tyout)) ptrs ]
+    else [::] (* absurd *)
   else [::]. (* absurd *)
 
 Definition isem_asm_res
-  (o : _No) (i : _In o) (m : _Mo) : itree E (_Out o * _Mo) :=
-  let xm := mkxm o m i in
+  (o : JNo) (i : JIn o) (m : MoT) : itree E (JOut o * MoT) :=
+  let xm := mkxm o m i (vi_ptrs i) in
   let* xm' := isem_asm q o xm in
-  Ret (xget_res o xm', xm').
+  Ret (xget_res o xm' (vi_ptrs i), xm').
 Arguments isem_asm_res : clear implicits.
 
-Definition _OoT (o : _No) (i : _In o) (m : _Mo) : itree Rnd (_Out o * _Mo) :=
-  let* ores := translateE (isem_asm_res o i m |> interp_Err) in
+Definition OoT (o : JNo) (i : JIn o) (m : MoT) : itree Rnd (JOut o * MoT) :=
+  let* ores := to_Rnd (isem_asm_res o i m |> interp_Err) in
   if ores is ESok res then Ret res
-  else Ret ([::], _mi) (* absurd *).
+  else Ret ([::], xmT). (* absurd *)
 
 Instance Target : OracleSystem JazzI :=
   {|
-    Mo := _Mo;
-    Oo := _OoT;
-    mi := _mi;
+    Mo := MoT;
+    Oo := OoT;
+    mi := xmT;
   |}.
 
 (* -------------------------------------------------------------------------- *)
@@ -439,35 +479,41 @@ Proof. exact: efn_fd_ok o. Qed.
   export_funname_get_fundef
   : core.
 
-Definition inv_mo : _Mo -> _Mo -> Prop.
+Definition sim : MoS -> MoT -> Prop.
 Proof using. Admitted.
 
-Definition inv_eq {X : Type} (x y : X * _Mo) : Prop :=
-  [/\ x.1 = y.1 & inv_mo x.2 y.2 ].
+Definition inv_eq {X : Type} : X * MoS -> X * MoT -> Prop :=
+  eqR (X := X) sim.
 
-Lemma inv_mo_mi : inv_mo _mi _mi.
+Lemma sim_mS_xmT : sim mS xmT.
 Proof using. Admitted.
 
-Lemma inv_mo_mem_equiv_mi ms mt :
-  inv_mo ms mt ->
-  mem_equiv mI ms.(asm_mem).
+Lemma sim_mem_equiv_mi ms mt :
+  sim ms mt ->
+  mem_equiv mS ms.
 Proof using. Admitted.
 
 Definition post_isem
-  (fn : funname) (ms mt : asmmem) (fs' : fstate) (xm' : asmmem) : Prop :=
-  exists xfd i,
-    let: fs := mkfs ms.(asm_mem) i in
-    let: xm := mkxm fn mt i in
+  (fn : funname)
+  (ptrs : seq pointer)
+  (ms : mem)
+  (mt : asmmem)
+  (fs' : fstate)
+  (xm' : asmmem) :
+  Prop :=
+  exists xfd vs,
+    let: fs := mkfs ms vs in
+    let: xm := mkxm fn mt vs ptrs in
     [/\ get_fundef q.(asm_funcs) fn = Some xfd
       , full_pre p q fn xfd fs xm
       & full_post cparams p q fn xfd fs xm fs' xm' ].
 
-Lemma post_isemP fn ms mt fs xm :
-  inv_mo ms mt ->
-  post_isem fn ms mt fs xm ->
+Lemma post_isemP fn ptrs ms mt fs xm :
+  sim ms mt ->
+  post_isem fn ptrs ms mt fs xm ->
   inv_eq
-    ([seq wseq_of_val v | v <- fvals fs], xm_with_mem (fmem fs) ms)
-    (xget_res fn xm, xm).
+    ([seq wseq_of_val v | v <- fvals fs], fmem fs)
+    (xget_res fn xm ptrs, xm).
 Proof using. Admitted.
 
 (* MOVE *)
@@ -522,25 +568,25 @@ by move=> s' t' hfin [].
 Qed.
 
 (* TODO missing hypotheses *)
-Lemma inv_mo_full_pre fn xfd i ms mt :
+Lemma sim_full_pre fn xfd i ptrs ms mt :
   get_fundef (asm_funcs q) fn = Some xfd ->
-  inv_mo ms mt ->
-  full_pre p q fn xfd (mkfs ms.(asm_mem) i) (mkxm fn mt i).
+  sim ms mt ->
+  full_pre p q fn xfd (mkfs ms i) (mkxm fn mt i ptrs).
 Proof using. Admitted.
 
-Lemma eutt_isem_post fn fd ms mt i :
+Lemma eutt_isem_post fn fd ms mt i ptrs :
   fn \in entries ->
   get_fundef p.(p_funcs) fn = Some fd ->
-  safe_uprog p fn (mkfs ms.(asm_mem) i) ->
-  res_defined p fn (mkfs ms.(asm_mem) i) ->
-  inv_mo ms mt ->
-  eutt (post_isem fn ms mt)
-    (isem_unit p fn (mkfs (asm_mem ms) i))
-    (isem_asm q fn (mkxm fn mt i)).
+  safe_uprog p fn (mkfs ms i) ->
+  res_defined p fn (mkfs ms i) ->
+  sim ms mt ->
+  eutt (post_isem fn ptrs ms mt)
+    (isem_unit p fn (mkfs ms i))
+    (isem_asm q fn (mkxm fn mt i ptrs)).
 Proof.
 move=> hfn hfd hsafe hdef hm.
 have [xfd hxfd heq] := correct_comp hfn hfd.
-have hpre := inv_mo_full_pre i hxfd hm.
+have hpre := sim_full_pre i ptrs hxfd hm.
 apply: eutt_subrel; last first.
 - apply: heq; first exact: hsafe.
   + exact: hdef.
@@ -549,30 +595,29 @@ move=> fs xm hpost; by exists xfd, i.
 Qed.
 
 Lemma eutt_isem_res o i ms mt :
-  inv_mo ms mt ->
+  sim ms mt ->
   eutt inv_eq (isem_unit_res o i ms) (isem_asm_res o i mt).
 Proof.
 move=> hm; apply: eutt_clo_bind.
 - apply: eutt_isem_post => //.
-  + exact/vi_safe/inv_mo_mem_equiv_mi/hm.
-  exact/vi_def/inv_mo_mem_equiv_mi/hm.
-move=> fs xm h; apply eutt_Ret; exact/(post_isemP hm h).
+  + exact/vi_safe/sim_mem_equiv_mi/hm.
+  exact/vi_def/sim_mem_equiv_mi/hm.
+move=> fs xm h; apply eutt_Ret; exact: post_isemP hm h.
 Qed.
 
-Theorem compiler_preserves o i m1 m2 :
-  inv_mo m1 m2 ->
-  eutt inv_eq (Source.(Oo) o i m1) (Target.(Oo) o i m2).
+Theorem compiler_preserves : simulating Source Target.
 Proof.
-move=> hm.
+exists sim; split; first exact: sim_mS_xmT.
+move=> o i m1 m2 hm.
 have [xfd [hgetq _ heq]] := [elaborate
   it_compile_prog_to_asmP haparams print_uprogP print_sprogP print_linearP
     hcomp (efn_export o)].
 (* TODO we could prove that we always get OK instead of using exec_rel *)
-apply: (eutt_clo_bind _ (UU := exec_rel inv_eq)).
-- exact/eutt_translateE/interp_exec_eutt/eutt_isem_res/hm.
+apply (eutt_clo_bind _ (UU := exec_rel inv_eq)).
+- apply/eutt_interp_RR/interp_exec_eutt_gen/eutt_isem_res/hm.
 move=> /= [[rs ms]|?] [[rt mt]|?] //=; last first.
-- move=> _; apply eutt_Ret; split=> //=; exact: inv_mo_mi.
-move=> [/= -> hm']; apply eutt_Ret; split=> //; exact: hm'.
+- move=> _; apply eutt_Ret; split=> //=; exact/sim_mS_xmT.
+move=> [/= -> hm']; apply eutt_Ret; split=> //; exact/hm'.
 Qed.
 
 End DEFS.
@@ -591,34 +636,41 @@ Context
   (export_encap : fn_encap \in entries)
   (export_decap : fn_decap \in entries)
   (p : uprog)
-  (fd_genkey_ok : get_fundef (p_funcs p) fn_genkey = Some fd_genkey)
-  (fd_encap_ok : get_fundef (p_funcs p) fn_encap = Some fd_encap)
-  (fd_decap_ok : get_fundef (p_funcs p) fn_decap = Some fd_decap)
-  (genkey_ok :
-    let: pk := WArray.empty pkbytes in
-    let: sk := WArray.empty skbytes in
-    safe_on p fn_genkey mI [:: Varr pk; Varr sk ]
-    /\ res_defined_on p fn_genkey mI [:: Varr pk; Varr sk ])
-  (encap_ok :
-    forall (pk : WArray.array pkbytes) (msg : WArray.array msgbytes),
-      arr_is_def pk ->
-      arr_is_def msg ->
-      safe_on p fn_encap mI [:: Varr pk; Varr msg ]
-      /\ res_defined_on p fn_encap mI [:: Varr pk; Varr msg ])
-  (decap_ok :
-    forall (sk : WArray.array skbytes) (ct : WArray.array ctbytes),
-      arr_is_def sk ->
-      arr_is_def ct ->
-      safe_on p fn_decap mI [:: Varr sk; Varr ct ]
-      /\ res_defined_on p fn_decap mI [:: Varr sk; Varr ct ])
 .
-
-Notation OracleSystem := (OracleSystem (R := R)) (only parsing).
 
 Definition pk0 := mkwvec pkbytes [::].
 Definition sk0 := mkwvec skbytes [::].
 Definition ct0 := mkwvec ctbytes [::].
 Definition msg0 := mkwvec msgbytes [::].
+
+Definition dummyp := WArray.empty pkbytes.
+Definition dummys := WArray.empty skbytes.
+Definition dummyc := WArray.empty ctbytes.
+Definition dummym := WArray.empty msgbytes.
+
+Context
+  (fd_genkey_ok : get_fundef (p_funcs p) fn_genkey = Some fd_genkey)
+  (fd_encap_ok : get_fundef (p_funcs p) fn_encap = Some fd_encap)
+  (fd_decap_ok : get_fundef (p_funcs p) fn_decap = Some fd_decap)
+  (ppk psk pct pmsg : pointer)
+  (genkey_ok :
+    let: args := [:: Varr dummyp; Varr dummys ] in
+    safe_on p fn_genkey mS args /\ res_defined_on p fn_genkey mS args)
+  (encap_ok :
+    forall (pk : WArray.array pkbytes),
+      let: args := [:: Varr dummyc; Varr dummym; Varr pk ] in
+      arr_is_def pk ->
+      safe_on p fn_encap mS args /\ res_defined_on p fn_encap mS args)
+  (decap_ok :
+    forall (ct : WArray.array ctbytes) (sk : WArray.array skbytes),
+      let: args := [:: Varr dummym; Varr sk; Varr ct ] in
+      arr_is_def ct ->
+      arr_is_def sk ->
+      safe_on p fn_decap mS args /\ res_defined_on p fn_decap mS args)
+.
+
+Notation OracleSystem := (OracleSystem (R := R)) (only parsing).
+
 
 #[local] Instance KEMP_of_JP : KEMParams :=
   {|
@@ -646,11 +698,52 @@ Section JKEM.
   Notation OutK := (Out (I := KEM)).
 
   Definition vi_GenKey : valid_input p efn_kg :=
-    {| vi_safe := genkey_ok.1; vi_def := genkey_ok.2; |}.
-  Definition vi_Encap (i : InK OEncap) : valid_input p efn_encap.
+    {|
+      _args := [:: Varr dummyp; Varr dummys ];
+      vi_safe := genkey_ok.1;
+      vi_def := genkey_ok.2;
+      vi_ptrs := [::];
+    |}.
+
+  Let mk_arr {n : positive} (s : wvec n) :=
+    Varr (rdflt (WArray.empty _) (WArray.fill n (wseq_of_wvec s))).
+
+  (* MOVE *)
+  Lemma fill_ok (n : positive) bytes :
+    Pos.to_nat n = size bytes ->
+    exists a, WArray.fill n bytes = ok a.
+  Proof.
+  move=> h; rewrite /WArray.fill -h eqxx /=.
+  suff : exists z a, WArray.fill_aux n bytes = ok (z, a).
+  - by move=> [z [a {}h]]; rewrite h; exists a.
+  have := WArray.fill_aux_ok (len := n) (bytes := bytes).
+  rewrite h => /(_ (le_n _)).
+  by case: WArray.fill_aux => // [[z a] ?] /=; exists z, a.
+  Qed.
+
+  Lemma arr_is_def_mk_arr (n : positive) (s : wvec n) :
+    arr_is_def (rdflt (WArray.empty _) (WArray.fill n (wseq_of_wvec s))).
+  Proof using.
+    have : Pos.to_nat n = size (s : wseq) by admit.
+    move=> /fill_ok [a h]; rewrite h /=.
+    rewrite /arr_is_def.
   Admitted.
-  Definition vi_Decap (i : InK ODecap) : valid_input p efn_decap.
-  Admitted.
+
+  Definition vi_Encap (i : InK OEncap) : valid_input p efn_encap :=
+    {|
+      _args := [:: Varr dummyc; Varr dummym; mk_arr i ];
+      vi_ptrs := [:: pmsg ];
+      vi_safe := (encap_ok (arr_is_def_mk_arr i)).1;
+      vi_def := (encap_ok (arr_is_def_mk_arr i)).2;
+    |}.
+
+  Definition vi_Decap (i : InK ODecap) : valid_input p efn_decap :=
+    {|
+      _args := [:: Varr dummym; mk_arr i.1; mk_arr i.2 ];
+      vi_ptrs := [:: pmsg; psk; pct ];
+      vi_safe := (decap_ok (arr_is_def_mk_arr i.2) (arr_is_def_mk_arr i.1)).1;
+      vi_def := (decap_ok (arr_is_def_mk_arr i.2) (arr_is_def_mk_arr i.1)).2;
+    |}.
 
   Let Oo_JKEM_GenKey
     (i : InK OGenKey) (m : Mo) : itree Rnd (OutK OGenKey * Mo) :=
@@ -690,11 +783,35 @@ End JKEM.
 Lemma simulating_JKEM P Q :
   simulating P Q ->
   simulating (KEM_of_Jazz P) (KEM_of_Jazz Q).
-Proof using. Admitted.
+Proof.
+move=> [sim hsim]; exists sim; split; first exact/hsim.(sim_mi).
+move=> [[] | pk | [sk ct]] m1 m2 hm.
+- apply: eutt_clo_bind; first exact: hsim.(sim_Oo) hm.
+  move=> [r m1'] [_ m2'] [/= <-] hm'.
+  by case: r => [| pk [| sk [|??]]]; apply eutt_Ret.
+- apply: eutt_clo_bind; first exact: hsim.(sim_Oo) hm.
+  move=> [r m1'] [_ m2'] [/= <-] hm'.
+  by case: r => [| ct [| msg [|??]]]; apply eutt_Ret.
+apply: eutt_clo_bind; first exact: hsim.(sim_Oo) hm.
+move=> [r m1'] [_ m2'] [/= <-] hm'.
+by case: r => [| msg [|??]]; apply eutt_Ret.
+Qed.
 
-Theorem mlkem_end_to_end q :
+Context
+  (q : asm_prog)
+  {lowering_options : Type}
+  (aparams : architecture_params lowering_options)
+  (haparams : h_architecture_params aparams)
+  (cparams : compiler_params lowering_options)
+  (print_uprogP : forall s p, cparams.(print_uprog) s p = p)
+  (print_sprogP : forall s p, cparams.(print_sprog) s p = p)
+  (print_linearP : forall s p, cparams.(print_linear) s p = p)
+  (hcomp : compile_prog_to_asm aparams cparams entries p = ok q)
+.
+
+Theorem mlkem_end_to_end :
   indcca_reduction (KEM_of_Jazz (Source p)) (KEM_of_Jazz (Target p q)).
-Proof using. Admitted.
+Proof. by apply/sim_indcca_adv/simulating_JKEM/compiler_preserves; eauto. Qed.
 
 End INSTANTIATION.
 
